Finished proof of correctness for messages
Now what's left to do is relate it to encoding/decoding nats, which I've
already started.
- Implementation of encode_nat
- encode_inv
- equal_message_decoding
- Possibly change the specification to take a hypothesis that gives an
upper bound on X, rather than an upper bound on the length of the
encoded list. This would require another lemma relating the length of
encoded lists to the size of X.

BrokenDevice/broken_device.v
@@ -7,7 +7,7 @@ Require Extraction.
 
 (** ** Definitions *)
 Module Definitions.
-Inductive bit := B0 | B1.
+Inductive bit := B1 | B0.
 
 Definition broken_list := list bool.
 Definition message := list bit.
@@ -15,7 +15,10 @@ Definition packet : Set := bit * bit * bit.
 Definition chunk : Set := bool * bool * bool.
 
 Fixpoint encode_nat (n : nat) : message. Admitted.
-Fixpoint decode_nat (x : message) : nat. Admitted.
+Fixpoint decode_nat (x : message) : nat := match x with
+  | [] => 0
+  | x :: xs => (if x then 1 else 0) + 2 * decode_nat xs
+  end.
 
 Fixpoint bools_to_chunks (p : broken_list) : list chunk :=  match p with
   | a :: b :: c :: rest => (a,b,c) :: bools_to_chunks rest
@@ -85,8 +88,8 @@ Definition decode_packet (p : packet) : message := match p with
     end.
 
 Fixpoint drop {A} (n : nat) (l : list A) : list A := match n, l with
-  | n  , []      => l
   | 0  , l       => l
+  | n  , []      => l
   | S n, x :: ls => drop n ls
   end.
 
@@ -104,8 +107,13 @@ Fixpoint decode (x : list packet) : message := match x with
 Definition anna (x : message) (p : broken_list) : message :=
   packets_to_message (encode x (bools_to_chunks p)).
 
+Definition anna_nat (X : nat) (p : broken_list) := anna (encode_nat X) p.
+
 Definition bruno (x : message) : message :=
   decode (message_to_packets x).
+
+Definition bruno_nat (x : message) : nat :=
+  decode_nat (bruno x).
 End Definitions.
 
 Module Examples.
@@ -135,7 +143,7 @@ Theorem list_two_induction {A} (P : list A -> Prop) :
   P [] -> 
   (forall a, P [a]) -> 
   (forall a b l, P l -> 
-                   P (a :: l) -> 
+                   (forall c, P (c :: l)) -> 
                    P (a :: b :: l)) ->
   (forall l, P l).
 Proof.
@@ -179,26 +187,108 @@ Qed.
 (** Two message are equal if they are the same elements, ignoring tailing zeros*)
 (** This definition is still kind of stupid, may adjust it to make the proofs easier *)
 Inductive equal_message : message -> message -> Prop :=
-  | equal_nil : 
-      equal_message [] []
-  | equal_cons : forall xs ys x y,
+  | equal_cons : forall xs ys x,
       equal_message xs ys ->
-      equal_message (x :: xs) (y :: ys)
-  | equal_tail_0 : forall xs ys,
-      equal_message xs ys ->
-      equal_message xs (ys ++ [B0])
-  | equal_symm : forall xs ys,
-      equal_message xs ys ->
-      equal_message ys xs.
+      equal_message (x :: xs) (x :: ys)
+  | equal_tail_0 : forall xs,
+      Forall (fun x => x = B0) xs ->
+      equal_message xs [].
 Hint Constructors equal_message : core.
 
-Example equal_ex : equal_message [B1; B0; B1] [B1; B0; B1; B0; B0; B0].
+Inductive prefix : message -> message -> Prop :=
+  | prefix_nil : forall ys,
+      length ys > 0 ->
+      prefix [] ys
+  | prefix_cons : forall xs ys x,
+      prefix xs ys ->
+      prefix (x::xs) (x::ys).
+Hint Constructors prefix : core.
+
+Definition prefix_or_equal m1 m2:=
+  prefix m1 m2 \/ equal_message m1 m2.
+
+Lemma equal_empty_zeros : forall msg,
+  equal_message msg [] ->
+ Forall (fun x => x = B0) msg.
 Proof.
-  assert (H : [B1; B0; B1; B0; B0; B0] = (([B1; B0; B1] ++ [B0]) ++ [B0]) ++ [B0]).
+  intros.
+  induction msg; auto.
+  inversion H; subst.
+  inversion H0; subst.
   auto.
-  rewrite H.
-  repeat apply equal_tail_0.
-  auto.
+Qed.
+
+Lemma equal_nil_cons : forall msg,
+  equal_message msg [] ->
+  equal_message (B0 :: msg) [].
+Proof.
+  intros.
+  destruct msg; auto.
+  constructor. constructor; auto.
+  inversion H. auto.
+Qed.
+
+Lemma empty_message_prefix : forall p,
+  equal_message (decode (encode [] p)) [].
+Proof.
+  intros.
+  induction p.
+  simpl. auto.
+  destruct a as [[a b] c]. destruct a, b, c; simpl; try apply IHp; try (repeat apply equal_nil_cons); auto.
+Qed.
+
+Lemma one_message_prefix : forall p a,
+  prefix_or_equal (decode (encode [a] p)) [a].
+Proof.
+  intros.
+  induction p as [| [[a' b'] c'] p IH].
+  simpl; left; auto.
+  remember (decode (encode [] p)) as l.
+  assert (Hz : Forall (fun x => x = B0) l). { apply equal_empty_zeros. subst. apply empty_message_prefix. }
+  destruct a, a', b', c'; simpl; auto; rewrite <- Heql; right; repeat constructor; auto.
+Qed.
+
+Theorem decoding_encoding_preserves_order : forall msg p,
+  prefix_or_equal (decode (encode msg p)) msg.
+Proof.
+  induction msg using list_two_induction; intros.
+  - right. apply empty_message_prefix.
+  - apply one_message_prefix.
+  - generalize dependent b. generalize dependent a. 
+    induction p as [| [[a' b'] c'] p IHp]; intros.
+    + left; constructor; simpl; lia. 
+    + destruct a', b', c', a, b; simpl;
+      solve [ apply IHp
+            | destruct (H B0 p) as [H1 | H2];
+              [left | right]; constructor; auto
+            | destruct (H B1 p) as [H1 | H2];
+              [left | right]; constructor; auto
+            | destruct (IHmsg p) as [H1 | H2];
+              [left | right]; constructor; auto].
+            
+Qed.
+
+Lemma prefix_len_less : forall m1 m2,
+  prefix m1 m2 -> length m1 < length m2.
+Proof.
+  intros. induction H; simpl; lia.
+Qed.
+
+Theorem decoding_length_equal : forall msg p,
+  prefix_or_equal (decode (encode msg p)) msg ->
+  length (decode (encode msg p)) >= length msg ->
+  equal_message (decode (encode msg p)) msg.
+Proof.
+  intros msg p H_pre H_len.
+  pose proof (prefix_len_less (decode (encode msg p)) msg).
+  destruct H_pre.
+  - apply H in H0. lia.
+  - auto.
+Qed.
+
+Example equal_ex : equal_message [B1; B0; B1; B0; B0; B0] [B1; B0; B1].
+Proof.
+  repeat constructor.
 Qed.
 
 Fixpoint count_broken (p : list chunk) := match p with
@@ -287,20 +377,27 @@ Qed.
 Definition message_preserved (N K L : nat) := forall x p, 
   length p = N ->
   count_broken (bools_to_chunks p) = K ->
-  length x = L ->
+  length x <= L ->
   equal_message (bruno (anna x p)) x.
 
-Lemma bools_to_chunks_length : forall p (m n : nat),
+Definition message_preserved_nat (N K L : nat) := forall X p, 
+  length p = N ->
+  count_broken (bools_to_chunks p) = K ->
+  length (encode_nat X) <= L ->
+  bruno_nat (anna_nat X p) = X.
+
+Fixpoint div3 (n : nat) := match n with
+  | S (S (S n')) => 1 + div3 n'
+  | _ => 0
+  end.
+
+Lemma bools_to_chunks_length : forall p (n : nat),
   length p = n ->
-  3 * m = n ->
-  length (bools_to_chunks p) = m.
+  length (bools_to_chunks p) = div3 n.
 Proof.
   intros.
   generalize dependent n.
-  generalize dependent m.
-  induction p using list_three_induction; intros; simpl in *; auto; try lia.
-  clear IHp0. clear IHp1.
-  rewrite (IHp (m-1) (n-3)); lia. 
+  induction p using list_three_induction; unfold div3; intros; subst; simpl; auto.
 Qed.
 
 Theorem correct_message_for_given_constraints :
@@ -317,9 +414,29 @@ Proof.
     pose proof (chunk_count_sumsto_count_broken l x y z Hcnt).
     lia. }
   pose proof (chunk_count_decoded_length msg l x y z Hcnt) as H_decoded_length.
+  apply decoding_length_equal. apply decoding_encoding_preserves_order. lia.
   (* Now we know that the length of the decoded message is at least 60 (the length of the original message). *)
   (* Next, we must show that any decoded message is either a prefix of the original message, or it is equal (possibly with tailing zeros). 
      Since we know that it cannot be a strict prefix since its length is >= 60, it must indeed be equal. *)
-Admitted.  
+Qed.
+
+Lemma encode_inv : forall X,
+  X = decode_nat (encode_nat X).
+Proof. Admitted.
+
+Lemma equal_message_decoding : forall m1 m2,
+  equal_message m1 m2 ->
+  decode_nat m1 = decode_nat m2.
+Proof. Admitted.
+
+Theorem correct_message_for_given_constraints_nat :
+  message_preserved_nat 150 40 60.
+  unfold message_preserved_nat.
+  intros.
+  unfold bruno_nat, anna_nat.
+  rewrite encode_inv.
+  apply equal_message_decoding.
+  apply correct_message_for_given_constraints; auto.
+Qed.
 
 End Verification.
